src/Std/Data/Iterators/Lemmas/Combinators/Monadic/TakeWhile.lean
@@ -9,16 +9,16 @@ import Std.Data.Iterators.Lemmas.Consumers.Monadic
 
 namespace Std.Iterators
 
-theorem IterM.step_takeWhileWithProof {α m β} [Monad m] [Iterator α m β]
+theorem IterM.step_takeWhileWithPostcondition {α m β} [Monad m] [Iterator α m β]
     {it : IterM (α := α) m β} {P} :
-    (it.takeWhileWithProof P).step = (do
+    (it.takeWhileWithPostcondition P).step = (do
       match ← it.step with
       | .yield it' out h => match ← (P out).operation with
-        | ⟨.up true, h'⟩ => pure <| .yield (it'.takeWhileWithProof P) out (.yield h h')
+        | ⟨.up true, h'⟩ => pure <| .yield (it'.takeWhileWithPostcondition P) out (.yield h h')
         | ⟨.up false, h'⟩ => pure <| .done (.rejected h h')
-      | .skip it' h => pure <| .skip (it'.takeWhileWithProof P) (.skip h)
+      | .skip it' h => pure <| .skip (it'.takeWhileWithPostcondition P) (.skip h)
       | .done h => pure <| .done (.done h)) := by
-  simp only [takeWhileWithProof, step, Iterator.step, internalState_toIterM]
+  simp only [takeWhileWithPostcondition, step, Iterator.step, internalState_toIterM]
   apply bind_congr
   intro step
   cases step using PlausibleIterStep.casesOn <;> rfl
@@ -32,11 +32,11 @@ theorem IterM.step_takeWhileM {α m β} [Monad m] [LawfulMonad m] [Iterator α m
         | .up false => pure <| .done (.rejected h True.intro)
       | .skip it' h => pure <| .skip (it'.takeWhileM P) (.skip h)
       | .done h => pure <| .done (.done h)) := by
-  simp only [takeWhileM, step_takeWhileWithProof]
+  simp only [takeWhileM, step_takeWhileWithPostcondition]
   apply bind_congr
   intro step
   cases step using PlausibleIterStep.casesOn
-  · simp only [Function.comp_apply, PostconditionT.operation_monadLift, PlausibleIterStep.yield,
+  · simp only [Function.comp_apply, PostconditionT.operation_lift, PlausibleIterStep.yield,
     PlausibleIterStep.done, bind_map_left]
     apply bind_congr
     rintro ⟨x⟩
